templates/flows/list_flow_upd_marking.v
@@ -14,62 +14,412 @@ Section list_flow_upd_marking.
   Definition list_flow_upd_marking n0 Nx Mk S I :=
     list_flow_upd f_incr n0 Nx Mk S I.
 
-  Lemma list_flow_upd_marking_invariants Key n R Nx Mk S I I' II' nk n0 In0:
+  Lemma list_flow_upd_marking_intfEq Key n R Nx Mk S I I' II' nk n0:
     let FI := λ I x, I !!! x in 
     (nx_key_rel Nx Key) →
     (nx_mk_closed Nx Mk (dom I)) →
-    (∀ x, x ∈ dom I → Mk !!! x = true → keyset (FI I x) = ∅) →
-    (∀ n1 n2, Nx !! n1 = Some n2 → dom (out_map (FI I n1)) = {[n2]}) →
-    (∀ n1 n2, n1 ∈ dom I' → Nx !! n1 = Some n2 → 
-      dom (out_map (FI I' n1)) = {[n2]}) →    
     (✓ ([^op set] x ∈ dom I, FI I x)) →
     (∀ x, x ∈ dom I → dom (FI I x) = {[x]}) →
-    (n0 ∈ dom I') → (n ∈ dom I') → (n0 ≠ n) →
+    (n0 ∈ dom I') → (n ∈ dom I') →
     (∀ x, x ∈ dom I' → Key !!! x ≤ Key !!! n) →
-    (∀ x, x ∈ dom I' ∖ {[n0]} → Key !!! n0 < Key !!! x) →
-    (FI I' n0 = In0) →
-    (FI I' n = inflow_insert_set (FI I n) n S) →
+    (FI I' n = inflow_map_set f_incr (FI I n) n S) →
     (dom I' ⊆ dom I) →
-    (∀ x, x ∈ dom I' ∖ {[n]} → Nx !! x ≠ None) →
-    (∀ x, x ∈ dom I' ∖ {[n0; n]} → FI I' x = 
-      outflow_insert_set (inflow_insert_set (FI I x) x S) (Nx !!! x) S) →
     (∀ x, x ∈ dom I' → dom (FI I' x) = {[x]}) →
-    (∀ x, x ∈ dom I' ∖ {[n0; n]} → keyset (FI I' x) = keyset (FI I x)) →
     ([^op set] x ∈ dom I', FI I x) = ([^op set] x ∈ dom I', FI I' x) →
     list_flow_upd_rec f_incr n R Nx Mk S I I' = Some (II', nk) →
-          ((dom II' ⊆ dom I)
-        ∧ (n0 ≠ nk)
-        ∧ (n0 ∈ dom II') 
-        ∧ (nk ∈ dom II')
-        ∧ (Mk !! nk = Some false)
-        ∧ (∀ x, x ∈ dom II' ∖ {[nk]} → Nx !! x ≠ None)
-        ∧ (∀ x, x ∈ dom II' → dom (FI II' x) = {[x]})
-        ∧ (([^op set] x ∈ dom II', FI I x) = ([^op set] x ∈ dom II', FI II' x))
-        ∧ (FI II' n0 = In0)
-        ∧ (FI II' nk = inflow_insert_set (FI I nk) nk S)
-        ∧ (∀ x, x ∈ dom II' ∖ {[n0;nk]} → FI II' x = 
-              outflow_insert_set (inflow_insert_set (FI I x) x S) (Nx !!! x) S)
-        ∧ (∀ x, x ∈ dom II' ∖ {[ n0; nk ]} → keyset (FI II' x) = keyset (FI I x))).
+        (([^op set] x ∈ dom II', FI I x) = ([^op set] x ∈ dom II', FI II' x)).
   Proof.
-    intros FI. 
-    intros Nx_key Hcl KS_mk Nx_dom Nx_dom0 VI Domm_I n0_in_I0 
-        n_in_I0 n0_neq_n Key_I0 Key_n0 Def_I0_n0 Def_I0_n Dom_I0_in_I 
-        Nx_x I0_x Domm_I0 KS_I' Heq Hflow.
-    repeat split.
-    - by apply (list_flow_upd_dom Key f_incr n R Nx Mk S I I' II' nk).
-    - by apply (list_flow_upd_neq Key f_incr n R Nx Mk S I I' II' nk).
-    - by apply (list_flow_upd_n0_dom f_incr n R Nx Mk S I I' II' nk).
-    - by apply (list_flow_upd_nk_dom f_incr n R Nx Mk S I I' II' nk).
-    - by apply (list_flow_upd_Mk_nk f_incr n R Nx Mk S I I' II' nk).
-    - by apply (list_flow_upd_Nx Key f_incr n R Nx Mk S I I' II' nk n0).
-    - by apply (list_flow_upd_domm Key f_incr n R Nx Mk S I I' II' nk).
-    - admit.
-    - by apply (list_flow_upd_II'_n0 Key f_incr n R Nx Mk S I I' II' nk n0).
-    - by apply (list_flow_upd_II'_nk f_incr n R Nx Mk S I I' II' nk).
-    - by apply (list_flow_upd_II' f_incr n R Nx Mk S I I' II' nk n0).
-    - admit.
-  Admitted.
+    intros FI. apply list_flow_upd_rec_ind; try done; last first.
+    - clear n R Nx Mk S I I'.
+      intros n R Nx Mk S I I0 n_in_R Hmk_n.
+      intros Nx_key Hcl VI Domm_I n0_in_I0 n_in_I0 Key_I0 Def_I0_n 
+        Dom_I0_in_I Domm_I0 Heq [= -> ->].
+      done.
+    - clear n R Nx Mk S I I'.
+      intros n R Nx Mk S I I0 n_in_R Hmk_n n1 Hnx_n In In' In1 In1' II I0'.
+      intros HInd Nx_key Hcl VI Domm_I n0_in_I0 n_in_I0 Key_I0 Def_I0_n 
+        Dom_I0_in_I Domm_I0 Heq Hflow.
+      assert (n1 ∉ dom I0) as n1_notin_I0.
+      { pose proof Nx_key n n1 Hnx_n as H'.
+        intros n1_in_I0. apply Key_I0 in n1_in_I0.
+        clear -H' n1_in_I0. lia. }
+      assert (dom I0' = dom I0 ∪ {[ n1 ]}) as Dom_I0'.
+      { rewrite /I0' /II.
+        repeat rewrite dom_insert_L.
+        clear -n_in_I0 n1_notin_I0.
+        set_solver. }
+      assert (n1 ∈ dom I) as n1_in_I.
+      { destruct Hcl as [_ [_ Hcl]].
+        by pose proof Hcl n n1 Hnx_n as H'. }  
+      assert (∀ x, x ∈ dom I0 → dom (FI (<[n:=In']> I0) x) = {[x]}) 
+        as Domm_II.
+      { intros x Hx. destruct (decide (n = x)) as [-> | Hxn].
+        - unfold FI. rewrite lookup_total_insert.
+          subst In'. rewrite flowint_outflow_map_set_domm.
+          subst In. rewrite Domm_I0; try done.
+        - unfold FI. rewrite lookup_total_insert_ne; try done.
+          rewrite Domm_I0; try done. }
+      apply HInd; try done; clear HInd.
+      + rewrite Dom_I0'. set_solver.
+      + rewrite Dom_I0'. set_solver.
+      + pose proof Nx_key n n1 Hnx_n as H'. 
+        rewrite Dom_I0'. intros x; rewrite elem_of_union.
+        intros [Hx | Hx].
+        * apply Key_I0 in Hx. clear -Hx H'. lia.
+        * assert (x = n1) as -> by (clear -Hx; set_solver).
+          clear; try done.
+      + rewrite /I0' /FI. rewrite lookup_total_insert. 
+        rewrite /In1'. by rewrite /In1.
+      + rewrite Dom_I0'. set_solver.
+      + rewrite Dom_I0'. intros x; rewrite elem_of_union.
+        intros [Hx | Hx].
+        * subst I0'. 
+          assert (x ≠ n1) as H'.
+          { clear -Hx n1_notin_I0. set_solver. }
+          unfold FI.
+          rewrite lookup_total_insert_ne; try done.
+          subst II.
+          apply Domm_II; try done.
+        * assert (x = n1) as -> by (clear -Hx; set_solver).
+          unfold FI. subst I0'.
+          rewrite lookup_total_insert.
+          subst In1'.
+          rewrite flowint_inflow_map_set_dom.
+          subst In1. rewrite Domm_I; try done.
+          clear; set_solver.
+      + rewrite Dom_I0'.
+        rewrite !big_opS_union; [try done | set_solver | set_solver].
+        rewrite !big_opS_singleton. 
+        all: try (clear -n_notin_I0; set_solver).
+        rewrite /I0'; rewrite /FI. rewrite lookup_total_insert.
+        rewrite /II.
+        assert (([^op set] y ∈ dom I0, FI (<[n1:=In1']> (<[n:=In']> I0)) y) = 
+                  ([^op set] y ∈ dom I0, FI (<[n:=In']> I0) y)) as Def_II.
+        { apply big_opS_ext. intros x Hx. unfold FI.
+          rewrite lookup_total_insert_ne. done.
+          clear -Hx n1_notin_I0. set_solver. }
+        rewrite Def_II.
+        assert (✓ ([^op set] y ∈ dom I0, FI I y)) as Valid_I.
+        { apply (flow_big_op_valid _ (dom I)); try done. }
+        assert (✓ ([^op set] y ∈ dom I0, FI I0 y)) as Valid_I0.
+        { apply leibniz_equiv_iff in Heq. rewrite <-Heq. try done. }
+        assert (✓ ([^op set] y ∈ dom I0, FI (<[n:=In']> I0) y)) as Valid_II.
+        { assert (([^op set] y ∈ dom I0, FI (<[n:=In']> I0) y) = 
+                    ([^op set] y ∈ dom I0 ∖ {[n]}, FI I0 y) ⋅ In') as ->.
+        { rewrite (big_opS_delete _ _ n); last done.
+          unfold FI at 1. rewrite lookup_total_insert.
+          rewrite intComp_comm.
+          assert (([^op set] y ∈ (dom I0 ∖ {[n]}), FI (<[n:=In']> I0) y) = 
+              ([^op set] y ∈ (dom I0 ∖ {[n]}), FI I0 y)) as ->.
+          { apply big_opS_ext. intros x Hx. unfold FI.
+            rewrite lookup_total_insert_ne. done.
+            clear -Hx; set_solver. }
+          done. }
 
+          apply (outflow_map_set_valid2
+                        (([^op set] y ∈ (dom I0 ∖ {[n]}), FI I0 y)) 
+                        (I0 !!! n) (In') f_incr n1 S).
+          - subst In'; try done.
+          - intros Hn1. rewrite flow_big_op_dom in Hn1.
+            destruct Hn1 as [x [Hx1 Hx2]].
+            rewrite Domm_I0 in Hx2; last first.
+            { clear -Hx1; set_solver. }
+            assert (n1 = x) as <- by (clear -Hx2; set_solver).
+            clear -n1_notin_I0 Hx1. set_solver.
+            apply (flow_big_op_valid _ (dom I0)); try done.
+            clear; set_solver.
+          - rewrite Domm_I0; try done.
+            assert (n1 ≠ n) as H'.
+            { clear -n1_notin_I0 n_in_I0.
+              set_solver. }
+            clear -H'; set_solver.
+          - intros H'. rewrite Domm_I0 in H'; try done.
+            clear -H'; set_solver.
+          - assert (([^op set] y ∈ (dom I0 ∖ {[n]}), FI I0 y) ⋅ I0 !!! n =
+                      ([^op set] y ∈ dom I0, FI I0 y)) as H'.
+            { rewrite (big_opS_delete _ (dom I0) n); try done.
+              unfold FI at 2. by rewrite intComp_comm. }
+            by rewrite H'. }
+        pose proof (flowint_insert_eq
+                      ([^op set] y ∈ dom I0, I !!! y)
+                      ([^op set] y ∈ dom I0, FI (<[n:=In']> I0) y)
+                      (I !!! n1) In1' n1 S) as Hpose.
+        assert (n1 ∈ dom (FI I n1)) as n1_in_In1.
+        { rewrite Domm_I; try done. clear; set_solver. }
+        assert (flowint_dom ([^op set] y ∈ dom I0, I !!! y) ≠ ∅) 
+          as Domm_I0_notEmpty.
+        { assert (n ∈ (flowint_dom ([^op set] y ∈ dom I0, (I !!! y)))) as H'.
+          { rewrite flow_big_op_dom; try done. exists n; split; try done.
+            rewrite Domm_I; last first.
+            { clear -n_in_I0 Dom_I0_in_I. set_solver. } 
+            clear; set_solver. }
+          clear -H'; set_solver. }
+        assert (flowint_dom ([^op set] y ∈ dom I0, (FI (<[n:=In']> I0) y)) = 
+                  flowint_dom ([^op set] y ∈ dom I0, (I !!! y))) as Domm_II_eq_I.
+        { assert ((flowint_dom ([^op set] y ∈ dom I0, (FI (<[n:=In']> I0) y))) ⊆ 
+                      (flowint_dom ([^op set] y ∈ dom I0, (I !!! y)))) as H'.
+          { intros n'. rewrite !flow_big_op_dom; try done.
+            intros [x [Hx1 Hx2]]. exists x. split; try done.
+            rewrite Domm_II in Hx2; try done. rewrite Domm_I; try done.
+            clear -Hx1 Dom_I0_in_I. set_solver. }
+          assert ((flowint_dom ([^op set] y ∈ dom I0, (I !!! y))) ⊆ 
+                    (flowint_dom ([^op set] y ∈ dom I0, (FI (<[n:=In']> I0) y)))) 
+                    as H''.
+          { intros n'. rewrite !flow_big_op_dom; try done.
+            intros [x [Hx1 Hx2]]. exists x. split; try done.
+            rewrite Domm_II. rewrite Domm_I in Hx2; try done.
+            clear -Hx1 Dom_I0_in_I. set_solver. done. }
+          clear -H' H''; set_solver. }
+        assert (([^op set] y ∈ dom I0, FI (<[n:=In']> I0) y) =
+          outflow_map_set f_incr ([^op set] y ∈ dom I0, I !!! y) n1 S) 
+          as H0'.
+        { apply intEq; try done. 
+          - unfold dom. rewrite Domm_II_eq_I. try done. 
+          - intros n'. unfold inf. rewrite outflow_map_set_inf.
+            assert (inf ([^op set] y ∈ dom I0, FI (<[n:=In']> I0) y) n'
+              ≡ default 0 
+                (inf_map ([^op set] y ∈ dom I0, FI (<[n:=In']> I0) y) !! n'))
+              as HL by try done.
+            assert (inf ([^op set] y ∈ dom I0, FI I y) n'
+              ≡ default 0 
+                (inf_map ([^op set] y ∈ dom I0, I !!! y) !! n')) 
+              as HR by try done.
+            rewrite <-HL. rewrite <-HR.
+            rewrite Heq.
+            assert (inf ([^op set] y ∈ dom I0, FI (<[n:=In']> I0) y) n' = 
+                      inf ([^op set] y ∈ dom I0, FI I0 y) n') as HI0.
+            { destruct (decide (n' ∈ 
+                          dom ([^op set] y ∈ dom I0, FI (<[n:=In']> I0) y))) 
+                as [Hn' | Hn'].
+              - rewrite flow_big_op_dom in Hn'; try done.
+                destruct Hn' as [n'' [n''_in_I0 n'_in_n'']].
+                rewrite Domm_II in n'_in_n''; try done.
+                assert (n' = n'') as <- by (clear -n'_in_n''; set_solver).
+                rewrite (flow_big_op_inf _ _ n'); try done.
+                + rewrite (flow_big_op_inf _ _ n'); try done.
+                  * clear HL HR. 
+                    assert (([^+ set] x ∈ (dom I0 ∖ {[n']}), 
+                              out (FI (<[n:=In']> I0) x) n')
+                            = ([^+ set] x ∈ (dom I0 ∖ {[n']}), 
+                              out (FI I0 x) n')) as Hout.
+                    { destruct (decide (n' = n)) as [-> | Hn'].
+                      - apply ccm_big_opS_ext. intros x Hx.
+                        unfold FI. rewrite lookup_total_insert_ne. done.
+                        clear -Hx; set_solver.  
+                      - assert (out (FI (<[n := In']> I0) n) n' 
+                                  = out (FI I0 n) n') as H'.
+                        { rewrite /FI. rewrite lookup_total_insert.
+                          rewrite /In' /In.
+                          assert (n' ≠ n1). 
+                          { clear -n''_in_I0 n1_notin_I0. set_solver. }
+                          unfold out. 
+                          rewrite outflow_map_set_out_map_ne; try done. }
+                        apply ccm_big_opS_ext. intros x Hx. unfold FI. 
+                        destruct (decide (x = n)) as [-> | Hxn]; try done.
+                        rewrite lookup_total_insert_ne; try done. }
+                    assert (inf (FI (<[n:=In']> I0) n') n' 
+                              = inf (FI I0 n') n') as Hin.
+                    { destruct (decide (n' = n)) as [-> | Hn'].
+                      - rewrite /FI. rewrite lookup_total_insert. 
+                        subst In'. unfold inf. 
+                        rewrite outflow_map_set_inf. by subst In.
+                      - rewrite /FI. 
+                        rewrite lookup_total_insert_ne; try done. }
+                    by rewrite Hin Hout.
+                  * rewrite Domm_I0; try done.
+                + rewrite Domm_II; try done.
+              - assert (n' ∉ dom ([^op set] y ∈ dom I0, FI I0 y)) as Hn''.
+                { unfold dom in Hn'. rewrite Domm_II_eq_I in Hn'.
+                  intros Hn''. rewrite flow_big_op_dom in Hn''; try done.
+                  destruct Hn'' as [x0 [Hx0 Hx00]].
+                  apply Hn'. rewrite flow_big_op_dom; try done.
+                  exists x0. split; try done.
+                  rewrite (Domm_I0 x0 Hx0) in Hx00.
+                  apply Dom_I0_in_I in Hx0.
+                  unfold FI in Domm_I.
+                  by rewrite (Domm_I x0 Hx0). }
+                unfold dom, flowint_dom in Hn''. 
+                unfold dom, flowint_dom in Hn'.
+                rewrite not_elem_of_dom in Hn'.
+                rewrite not_elem_of_dom in Hn''.
+                unfold inf. rewrite Hn' Hn''. by simpl. }
+            by rewrite HI0.
+          - rewrite Heq. intros n'.
+            destruct (decide (n' ∈ 
+                dom ([^op set] y ∈ dom I0, FI (<[n:=In']> I0) y))) 
+                as [Hn' | Hn'].
+            + rewrite intValid_in_dom_not_out; try done.
+              rewrite intValid_in_dom_not_out; try done.
+              apply outflow_map_set_valid; try done.
+              intros Hn1. rewrite flow_big_op_dom in Hn1; try done.
+              destruct Hn1 as [x0 [Hx0 Hx00]].
+              rewrite (Domm_I0 x0 Hx0) in Hx00.
+              clear -Hx0 Hx00 n1_notin_I0. set_solver.
+              assert (n ∈ dom ([^op set] x ∈ dom I0, FI I0 x)) as H'.
+              { rewrite flow_big_op_dom; try done. exists n.
+                rewrite (Domm_I0 n n_in_I0). split; try done.
+                clear; set_solver. } clear -H'; set_solver.
+              rewrite flowint_outflow_map_set_domm. 
+              rewrite flow_big_op_dom; try done.
+              rewrite flow_big_op_dom in Hn'; try done.
+              destruct Hn' as [x0 [Hx0 Hx00]].
+              destruct (decide (x0 = n)) as [-> | Hxn].
+              * unfold FI in Hx00. rewrite lookup_total_insert in Hx00.
+                rewrite /In' in Hx00.
+                rewrite flowint_outflow_map_set_domm in Hx00.
+                rewrite /In in Hx00.
+                exists n; split; try done.
+              * unfold FI in Hx00. 
+                rewrite lookup_total_insert_ne in Hx00; try done.
+                exists x0; split; try done.
+            + destruct (decide (n' = n1)) as [-> | Hn1'].
+              * apply nzmap_eq. intros k'. 
+                destruct (decide (k' ∈ S)) as [Hk' | Hk'].
+                ** rewrite outflow_lookup_total_map_set; try done.
+                   rewrite !flow_big_op_out; try done.
+                   { rewrite (ccm_big_opS_delete _ _ n); try done.
+                     rewrite (ccm_big_opS_delete _ (dom I0) n); try done.
+                     unfold ccmop, ccm_op. simpl.
+                     rewrite !lookup_total_lifting.
+                     unfold ccmop, ccm_op. simpl. unfold nat_op.
+                     unfold FI at 1. rewrite lookup_total_insert.
+                     rewrite {1}/In'. rewrite outflow_lookup_total_map_set.
+                     assert (([^+ set] y ∈ (dom I0 ∖ {[n]}), 
+                                out (FI (<[n:=In']> I0) y) n1) =
+                             ([^+ set] y ∈ (dom I0 ∖ {[n]}), 
+                                out (FI I0 y) n1)) as ->.
+                     { apply ccm_big_opS_ext. intros x Hx. unfold FI. 
+                       rewrite lookup_total_insert_ne; try done.
+                       clear -Hx; set_solver. }
+                     rewrite /In. rewrite -/(FI I0 n).
+                     rewrite /f_incr /ccmop /nat_op. 
+                     set a := out (FI I0 n) n1 !!! k'.
+                     set b := ([^+ set] y ∈ (dom I0 ∖ {[n]}), out (FI I0 y) n1) 
+                                                                         !!! k'.
+                     clear; lia. done. }
+                   { intros Hn1. rewrite flow_big_op_dom in Hn1; try done.
+                     destruct Hn1 as [x [Hx1 Hx2]].
+                     rewrite Domm_I0 in Hx2; try done.
+                     assert (n1 = x) as -> by (clear -Hx2; set_solver).
+                     clear -Hx1 n1_notin_I0. try done. }
+                ** rewrite outflow_lookup_total_map_set_ne; try done.
+                   rewrite !flow_big_op_out; try done.
+                   { rewrite (ccm_big_opS_delete _ _ n); try done.
+                     rewrite (ccm_big_opS_delete _ (dom I0) n); try done.
+                     unfold ccmop, ccm_op. simpl.
+                     rewrite !lookup_total_lifting.
+                     unfold FI at 1. rewrite lookup_total_insert.
+                     rewrite {1}/In'. 
+                     rewrite outflow_lookup_total_map_set_ne; try done.
+                     assert (([^+ set] y ∈ (dom I0 ∖ {[n]}), 
+                                out (FI (<[n:=In']> I0) y) n1) = 
+                             ([^+ set] y ∈ (dom I0 ∖ {[n]}), 
+                                out (FI I0 y) n1)) as ->.
+                     { apply ccm_big_opS_ext. intros x Hx. unfold FI. 
+                       rewrite lookup_total_insert_ne; try done.
+                       clear -Hx; set_solver. }
+                     by rewrite ccm_comm. }
+                   { intros Hn1. rewrite flow_big_op_dom in Hn1; try done.
+                     destruct Hn1 as [x [Hx1 Hx2]].
+                     rewrite Domm_I0 in Hx2; try done.
+                     assert (n1 = x) as -> by (clear -Hx2; set_solver).
+                     clear -Hx1 n1_notin_I0. try done. }
+              * unfold out at 2.
+                rewrite outflow_map_set_out_map_ne; try done.
+                fold (out ([^op set] x ∈ dom I0, FI I0 x) n').
+                rewrite !flow_big_op_out; try done; last first.
+                { intros Hn2'. rewrite flow_big_op_dom in Hn2'; try done. 
+                  destruct Hn2' as [x0 [Hx0 Hx00]].
+                  apply Hn'. apply flow_big_op_dom; try done.
+                  rewrite (Domm_I0 x0 Hx0) in Hx00.
+                  assert (n' = x0) as -> by (clear -Hx00; set_solver).
+                  exists x0. unfold FI. destruct (decide (x0 = n)) as [-> | Hx0n].
+                  - rewrite lookup_total_insert. rewrite /In'.
+                    rewrite flowint_outflow_map_set_domm. rewrite /In.
+                    rewrite (Domm_I0 n n_in_I0). split; try done.
+                  - rewrite lookup_total_insert_ne; try done.
+                    rewrite (Domm_I0 x0 Hx0). split; try done. }
+                apply ccm_big_opS_ext. intros x Hx.
+                destruct (decide (x = n)) as [-> | Hxn].
+                ** unfold FI. rewrite lookup_total_insert.
+                   rewrite /In'. unfold out.
+                   by rewrite outflow_map_set_out_map_ne.
+                ** unfold FI. rewrite lookup_total_insert_ne; try done. }
+        assert (In1' = inflow_map_set f_incr (I !!! n1) n1 S) as H0''.
+        { rewrite /In1' /In1. try done. }
+        assert (✓ (([^op set] y ∈ dom I0, FI I y) ⋅ (FI I n1))) as H0'''.
+        { assert (dom I0 ∪ {[ n1 ]} ⊆ dom I) as Hsub.
+          { clear -n1_in_I Dom_I0_in_I. set_solver. }
+          pose proof (flow_big_op_valid _ _ (dom I0 ∪ {[n1]}) Hsub VI) as H'.
+          rewrite big_opS_union in H'.
+          by rewrite big_opS_singleton in H'.
+          clear -n1_notin_I0. set_solver. }
+        apply Hpose; try done. 
+  Qed.
+
+  Lemma list_flow_upd_marking_KS Key n R Nx Mk S I I' II' nk n0:
+    let FI := λ I x, I !!! x in 
+    (nx_key_rel Nx Key) →
+    (nx_mk_closed Nx Mk (dom I)) →
+    (∀ x, x ∈ dom I ∖ {[n0]} → S ## keyset (FI I x)) →
+    (n ∈ dom I') → (dom I' ⊆ dom I) →
+    (∀ x, x ∈ dom I' → Key !!! x ≤ Key !!! n) →
+    (FI I' n = inflow_map_set f_incr (FI I n) n S) →
+    (∀ x, x ∈ dom I' ∖ {[n0; n]} → keyset (FI I' x) = keyset (FI I x)) →
+    list_flow_upd_rec f_incr n R Nx Mk S I I' = Some (II', nk) →
+      (∀ x, x ∈ dom II' ∖ {[n0; nk]} → keyset (FI II' x) = keyset (FI I x)).
+  Proof.
+    intros FI. apply list_flow_upd_rec_ind; try done; last first.
+    - clear n R Nx Mk S I I'.
+      intros n R Nx Mk S I I0 n_in_R Hmk_n.
+      intros Nx_key Hcl Disj_KS n_in_I0 Dom_I0_in_I Key_I0 Def_I0_n 
+        KS_x [= -> ->].
+      done.
+    - clear n R Nx Mk S I I'.
+      intros n R Nx Mk S I I0 n_in_R Hmk_n n1 Hnx_n In In' In1 In1' II I0'.
+      intros HInd Nx_key Hcl Disj_KS n_in_I0 Dom_I0_in_I Key_I0 Def_I0_n 
+        KS_x Hflow.
+      assert (n1 ∉ dom I0) as n1_notin_I0.
+      { pose proof Nx_key n n1 Hnx_n as H'.
+        intros n1_in_I0. apply Key_I0 in n1_in_I0.
+        clear -H' n1_in_I0. lia. }
+      assert (dom I0' = dom I0 ∪ {[ n1 ]}) as Dom_I0'.
+      { rewrite /I0' /II.
+        repeat rewrite dom_insert_L.
+        clear -n_in_I0 n1_notin_I0.
+        set_solver. }
+      assert (n1 ∈ dom I) as n1_in_I.
+      { destruct Hcl as [_ [_ Hcl]].
+        by pose proof Hcl n n1 Hnx_n as H'. }  
+      apply HInd; try done.
+      + rewrite Dom_I0'. clear; set_solver.
+      + rewrite Dom_I0'. clear -Dom_I0_in_I n1_in_I. set_solver.
+      + pose proof Nx_key n n1 Hnx_n as H'. 
+        rewrite Dom_I0'. intros x; rewrite elem_of_union.
+        intros [Hx | Hx].
+        * apply Key_I0 in Hx. clear -Hx H'. lia.
+        * assert (x = n1) as -> by (clear -Hx; set_solver).
+          clear; try done.
+      + by rewrite /I0' /FI lookup_total_insert /In1' /In1.
+      + intros x Hx; rewrite Dom_I0' elem_of_difference in Hx.
+        destruct Hx as [Hx1 Hx2]. rewrite elem_of_union in Hx1.
+        destruct Hx1 as [Hx1 | Hx1]; last first.
+        { clear -Hx1 Hx2; set_solver. }
+        destruct (decide (x = n)) as [-> | Hxn]; last first.
+        { rewrite /I0' /FI /II !lookup_total_insert_ne; try done. 
+          apply KS_x. clear -Hx1 Hx2 Hxn; set_solver. clear -Hx2; set_solver. }
+        rewrite /I0' /FI /II. 
+        rewrite lookup_total_insert_ne; last first. { clear -Hx2; set_solver. }
+        rewrite lookup_total_insert /In' /In.
+        rewrite /keyset. rewrite outflow_insert_set_insets.
+        rewrite outflow_insert_set_outsets. rewrite /FI in Def_I0_n.
+        rewrite Def_I0_n. rewrite inflow_insert_set_outsets.
+        rewrite inflow_insert_set_insets.
+        assert (n ∈ dom I ∖ {[n0]}) as H'.
+        { clear -Hx1 Hx2 Dom_I0_in_I. set_solver. }
+        apply Disj_KS in H'. rewrite /keyset /FI in H'.
+        clear -H'. set_solver.
+  Qed.
   
   Lemma marking_flow_upd_summary Key n0 Nx Mk S I res n1:
     let FI := λ I x, I !!! x in 
@@ -81,8 +431,12 @@ Section list_flow_upd_marking.
     (✓ ([^op set] x ∈ dom I, FI I x)) →
     (∀ x, x ∈ dom I → dom (FI I x) = {[x]}) →
     (n0 ∈ dom I) →
+    (S ≠ ∅) →
+    (∀ x, x ∈ dom I ∖ {[n0]} → S ## keyset (FI I x)) →
+    (*
     (S ⊆ insets (FI I n0)) →
     (S ## outsets (FI I n0)) →
+    *)
     list_flow_upd_marking n0 Nx Mk S I = res →
       ∃ II nk, 
         res = Some (II, nk)
@@ -100,26 +454,16 @@ Section list_flow_upd_marking.
       ∧ (FI II nk = inflow_insert_set (FI I nk) nk S)
       ∧ (∀ x, x ∈ dom II ∖ {[ n0; nk ]} → FI II x = 
               outflow_insert_set (inflow_insert_set (FI I x) x S) (Nx !!! x) S)
-      ∧ (keyset (FI II n0) = keyset (FI I n0) ∖ S)
+      (* ∧ (keyset (FI II n0) = keyset (FI I n0) ∖ S) *)
       ∧ (∀ x, x ∈ dom II ∖ {[ n0; nk ]} → keyset (FI II x) = keyset (FI I x)).
   Proof.
-    intros FI Nx_key Hcl KS_mk Nx_dom Hnx_n0 VI Domm_I n0_in_I 
-      Insets_S Outsets_S Hflow.
+    intros FI Nx_key Hcl KS_mk Nx_dom Hnx_n0 VI Domm_I n0_in_I S_nonempty
+      Disj_KS Hflow.
     unfold list_flow_upd_marking, list_flow_upd in Hflow.
     rewrite Hnx_n0 in Hflow. 
     set In1 := inflow_map_set f_incr (I !!! n1) n1 S.
     set In0 := outflow_map_set f_incr (I !!! n0) n1 S.
     set I': gmap Node (multiset_flowint_ur nat) := {[n1 := In1; n0 := In0]}.
-    (*
-    assert (In1 = inflow_map_set (λ _ x : nat, x + 1) (I !!! n1) n1 S) 
-      as Def_In1 by done.
-    assert (In0 = outflow_map_set (λ _ x : nat, x + 1) (I !!! n0) n1 S) 
-      as Def_In0 by done.
-    assert (I' = {[n1 := In1; n0 := In0]}) as Def_I' by done.
-    rewrite <-Def_In1 in Hflow.
-    rewrite <-Def_In0 in Hflow.
-    rewrite <-Def_I' in Hflow.
-    *)
     rewrite -/In1 -/In0 -/I' in Hflow.
     assert (dom I' = {[n0; n1]}) as Dom_I' by set_solver.
     assert (n1 ∈ dom I') as n1_in_I' by set_solver.
@@ -127,7 +471,9 @@ Section list_flow_upd_marking.
     { destruct Hcl as [_ [_ Hcl]]. 
       by apply (Hcl n0). }
     assert (n0 ≠ n1) as n0_neq_n1.
-    { admit. }
+    { pose proof Nx_key n0 n1 Hnx_n0. 
+      destruct (decide (n0 = n1)) as [-> | ]; try done.
+      lia. }
     assert (dom I = (dom I ∖ {[n0]}) ∪ dom I') as H'.
     { rewrite Dom_I'.
       assert ((dom I ∖ {[n0]}) ∪ {[n0; n1]} ⊆ dom I) as H'.
@@ -185,9 +531,6 @@ Section list_flow_upd_marking.
     assert (I' !!! n0 = In0) as Def_I'_n0.
     { subst I'. rewrite lookup_total_insert_ne; try done.
       rewrite lookup_total_insert; done. }      
-    assert (([^op set] x ∈ dom I', FI I x) = 
-                ([^op set] x ∈ dom I', FI I' x)) as Heq.
-    { admit. }
     assert (✓ (I !!! n0 ⋅ I !!! n1)) as VI'.
     { assert ({[n0; n1]} ⊆ dom I) as Hsub.
       { clear -n1_in_I n0_in_I' Dom_I'_in_I. set_solver. }
@@ -195,70 +538,95 @@ Section list_flow_upd_marking.
       rewrite big_opS_union in VI'.
       rewrite !big_opS_singleton in VI'.
       by unfold FI in VI'. clear -n0_neq_n1. set_solver. }
-
-    assert (insets In0 = insets (I !!! n0)) as H1'.
-    { by rewrite outflow_insert_set_insets. }
+    assert (([^op set] x ∈ dom I', FI I x) = 
+                ([^op set] x ∈ dom I', FI I' x)) as Heq.
+    { rewrite Dom_I'. 
+      rewrite !big_opS_union; [| (clear -n0_neq_n1; set_solver)..].
+      rewrite !big_opS_singleton.
+      rewrite /I'. unfold FI.
+      rewrite lookup_total_insert_ne; try done.
+      rewrite !lookup_total_insert.
+      rewrite /In0 /In1. 
+      apply (flowint_insert_eq _ _ _ _ n1 S); try done.
+      - rewrite Domm_I; set_solver.
+      - rewrite Domm_I; clear -n0_in_I' Dom_I'_in_I; set_solver. }
+    
+    assert (nzmap_map_set f_incr S (out (I !!! n0) n1) ≠ 0) as HS'.
+    { apply set_choose_L in S_nonempty.
+      destruct S_nonempty as [xs HS].
+      intros H'. rewrite nzmap_eq in H'.
+      pose proof H' xs as H'. rewrite nzmap_lookup_empty in H'.
+      rewrite nzmap_lookup_total_map_set /f_incr in H'; try done.
+      rewrite /ccmop /nat_op /ccmunit /= /nat_unit in H'. 
+      clear -H'. lia. }
     assert (dom (out_map In0) = dom (out_map (FI I n0))) as Domout_map.
-    { rewrite /In0. unfold outflow_insert_set, outflow_map_set.
-      simpl. apply leibniz_equiv. rewrite nzmap_dom_insert_nonzero.
-      unfold FI. rewrite (Nx_dom n0 n1 Hnx_n0).
-      clear; set_solver.
-      (*
-      destruct Outset_k as [k H'']. 
-      intros Hn. rewrite nzmap_eq in Hn.
-      pose proof Hn k as Hn.
-      rewrite nzmap_lookup_total_map_set_ne in Hn; last first.
-      clear -H''; set_solver.
-      unfold ccmunit, ccm_unit in Hn. simpl in Hn.
-      unfold lift_unit in Hn.
-      rewrite nzmap_lookup_empty in Hn.
-      destruct H'' as [H'' _].
-      unfold outset in H''. rewrite nzmap_elem_of_dom_total in H''.
-      unfold FI in H''. clear -Hn H''; try done.
-      *) admit. }
-    assert (outsets In0 = outsets (I !!! n0) ∪ S) as H1''.
-    { unfold outsets.
-      pose proof (Nx_dom n0 n1 Hnx_n0) as Nx_dom.
-      unfold FI in Nx_dom. rewrite Domout_map.
-      rewrite Nx_dom. apply leibniz_equiv. rewrite !big_opS_singleton.
-      rewrite /In0. rewrite outflow_insert_set_outset; try done. }
-    (*
-    assert (S  insets (I !!! n1)) as Insets_S1.
-    { intros k Hk. unfold insets. 
-      rewrite (Domm_I n1 n1_in_I).
-      rewrite big_opS_singleton.
-      apply (flowint_inset_step (I !!! n0) (I !!! n1)); try done.
-      - unfold FI in Domm_I. rewrite (Domm_I n1 n1_in_I).
-        clear; set_solver.
-      - unfold outset. rewrite nzmap_elem_of_dom_total; try done.
-        (*
-        rewrite Outset_S. unfold ccmunit, ccm_unit. simpl. 
-        unfold nat_unit. clear; lia. done. *)
-        admit. }
-    *)
+    { rewrite /In0 /outflow_insert_set /outflow_map_set.
+      simpl. apply leibniz_equiv. rewrite nzmap_dom_insert_nonzero; try done.
+      rewrite /FI (Nx_dom n0 n1 Hnx_n0).
+      clear; set_solver. }
     assert (∀ x : Node, x ∈ dom I' ∖ {[n0; n1]} →  
       keyset (I' !!! x) = keyset (I !!! x)) as KS_I'.
     { rewrite Dom_I'. intros x Hx. clear -Hx; set_solver. }  
 
+    (*
+    assert (insets In0 = insets (I !!! n0)) as Insets_In0.
+    { by rewrite outflow_insert_set_insets. }
+    assert (outsets In0 = outsets (I !!! n0) ∪ S) as Outsets_In0.
+    { unfold outsets.
+      pose proof (Nx_dom n0 n1 Hnx_n0) as Nx_dom.
+      unfold FI in Nx_dom. rewrite Domout_map Nx_dom.
+      apply leibniz_equiv. rewrite !big_opS_singleton.
+      rewrite /In0. rewrite outflow_insert_set_outset; try done. }
     assert (keyset In0 = keyset (I !!! n0) ∖ S) as KS_n0.
-    { unfold keyset. rewrite H1' H1''. 
+    { unfold keyset. rewrite Insets_In0 Outsets_In0.
       apply set_eq_subseteq.
+      split. 
       split; clear -Insets_S Outsets_S; set_solver. }
+    *)
     assert (∀ n1 n2, n1 ∈ dom I' → Nx !! n1 = Some n2 → 
       dom (out_map ((I' !!! n1: multiset_flowint_ur nat))) = {[n2]}) as Nx_dom'.
-    { admit. }
-      
+    { intros n2 n3. rewrite Dom_I'. rewrite elem_of_union.
+      intros [Hn2 | Hn2].
+      - assert (n2 = n0) as -> by (clear -Hn2; set_solver).
+        rewrite Hnx_n0. intros [=<-]. rewrite /I'.
+        rewrite lookup_total_insert_ne; try done.
+        rewrite lookup_total_insert /In0. 
+        apply set_eq_subseteq. split.
+        + intros x Hx. rewrite nzmap_elem_of_dom_total in Hx.
+          rewrite /outflow_map_set /= in Hx.
+          destruct (decide (x = n1)) as [-> | Hxn1]; try done.
+          { clear; set_solver. }
+          rewrite nzmap_lookup_total_insert_ne in Hx; try done.
+          rewrite -nzmap_elem_of_dom_total2 in Hx. apply dec_stable in Hx.
+          rewrite /FI in Nx_dom.
+          rewrite (Nx_dom n0 n1 Hnx_n0) in Hx.
+          clear -Hxn1 Hx; set_solver. 
+        + intros x Hx. assert (x = n1) as -> by (clear -Hx; set_solver).
+          rewrite nzmap_elem_of_dom_total. rewrite /outflow_map_set /=.
+          rewrite nzmap_lookup_total_insert; try done.
+      - assert (n2 = n1) as -> by (clear -Hn2; set_solver).
+        rewrite /I'. rewrite lookup_total_insert /In1 /=.
+        apply Nx_dom. }
+    assert (∀ x, x ∈ dom I' ∖ {[n0; n1]} → Mk !! x = Some true) as Mk_x.
+    { intros x Hx; rewrite Dom_I' in Hx. clear -Hx; set_solver. }
     
+    set R := dom I ∖ {[n0]}.
     
-    pose proof list_flow_upd_marking_invariants Key n1 (dom I ∖ {[n0]}) Nx Mk S 
-      I I' II nk n0 In0 Nx_key Hcl KS_mk Nx_dom Nx_dom' VI Domm_I 
-      n0_in_I' n1_in_I' n0_neq_n1 Key_I' Key_n0 Def_I'_n0 Def_I'_n 
-      Dom_I'_in_I Nx_x I'_x Domm_I' KS_I' Heq Hflow1 
-      as [HInv1 [HInv2 [HInv3 [HInv4 [HInv5 
-            [HInv6 [HInv7 [HInv8 [HInv9 [HInv10 [HInv11 HInv13]]]]]]]]]]].
-
-    exists II, nk. repeat (split; try done). admit. admit.
-    unfold FI at 1. by rewrite HInv9.
-  Admitted.
+    exists II, nk. repeat split; try done.
+    - by apply (list_flow_upd_dom Key f_incr n1 R Nx Mk S I I' II nk).
+    - by apply (list_flow_upd_n0_dom f_incr n1 R Nx Mk S I I' II nk).
+    - by apply (list_flow_upd_nk_dom f_incr n1 R Nx Mk S I I' II nk).
+    - by apply (list_flow_upd_neq Key f_incr n1 R Nx Mk S I I' II nk).
+    - by apply (list_flow_upd_Mk_nk f_incr n1 R Nx Mk S I I' II nk).
+    - by apply (list_flow_upd_Mk f_incr n1 R Nx Mk S I I' II nk).
+    - by apply (list_flow_upd_Nx Key f_incr n1 R Nx Mk S I I' II nk n0).
+    - by apply (list_flow_upd_Key_n0 Key f_incr n1 R Nx Mk S I I' II nk n0).
+    - by apply (list_flow_upd_domm Key f_incr n1 R Nx Mk S I I' II nk).
+    - by apply (list_flow_upd_marking_intfEq Key n1 R Nx Mk S I I' II nk n0).
+    - by apply (list_flow_upd_II'_n0 Key f_incr n1 R Nx Mk S I I' II nk n0).
+    - by apply (list_flow_upd_II'_nk f_incr n1 R Nx Mk S I I' II nk).
+    - by apply (list_flow_upd_II' f_incr n1 R Nx Mk S I I' II nk n0).
+    - by apply (list_flow_upd_marking_KS Key n1 R Nx Mk S I I' II nk n0).
+  Qed.
   
 End list_flow_upd_marking.
